Batteries/Data/List/Perm.lean
@@ -314,10 +314,12 @@ theorem Perm.inter {l₁ l₂ t₁ t₂ : List α} (p₁ : l₁ ~ l₂) (p₂ : 
 
 end DecidableEq
 
-theorem Perm.join_congr :
-    ∀ {l₁ l₂ : List (List α)} (_ : List.Forall₂ (· ~ ·) l₁ l₂), l₁.join ~ l₂.join
+theorem Perm.flatten_congr :
+    ∀ {l₁ l₂ : List (List α)} (_ : List.Forall₂ (· ~ ·) l₁ l₂), l₁.flatten ~ l₂.flatten
   | _, _, .nil => .rfl
-  | _ :: _, _ :: _, .cons h₁ h₂ => h₁.append (Perm.join_congr h₂)
+  | _ :: _, _ :: _, .cons h₁ h₂ => h₁.append (Perm.flatten_congr h₂)
+
+@[deprecated (since := "2024-10-15")] alias Perm.join_congr := Perm.flatten_congr
 
 theorem perm_insertP (p : α → Bool) (a l) : insertP p a l ~ a :: l := by
   induction l with simp [insertP, insertP.loop, cond]
